LoL/InfNonDet.lean
@@ -1,0 +1,115 @@
+import Mathlib.Logic.Function.Basic
+import Aesop
+import LoL.QuotientExtra
+import LoL.Meta
+
+
+universe u v w
+
+structure NonDetM (α : Type u) where
+  tp : Type v
+  val : tp → α
+
+variable {α : Type u} {β : Type v}
+
+def NonDetM.pure (x : α) : NonDetM α := ⟨Unit, fun _ => x⟩
+
+def NonDetM.bind (x : NonDetM α) (f : α → NonDetM β) : NonDetM β :=
+  ⟨Σ (t : x.tp), f (x.val t) |>.tp, fun b => f (x.val b.fst) |>.val b.snd⟩
+
+instance : Monad NonDetM where
+  pure := NonDetM.pure
+  bind := NonDetM.bind
+
+
+abbrev NonDetM.choose (τ : Type u) : NonDetM τ := ⟨τ, id⟩
+abbrev NonDetM.assume (as : Prop) : NonDetM Unit := ⟨PLift as, fun _ => ()⟩
+
+def NonDetM.run (x : NonDetM α) [Inhabited x.tp] : α := x.val default
+
+abbrev succ (x : Int) : NonDetM Int :=
+  do
+    let y <- NonDetM.choose Int
+    NonDetM.assume (y > x)
+    let z <- NonDetM.choose Int
+    NonDetM.assume (z < x)
+    return y + z
+
+example (P : _ -> Prop) i : P ((succ i)) := by
+  dsimp [succ, bind, pure, NonDetM.choose, NonDetM.assume, NonDetM.pure, NonDetM.bind]
+  -- simp [StateT.bind, StateT.get, pure, NonDetM.pure, liftM, monadLift, MonadLift.monadLift]
+  -- simp [succ', bind, pure, NonDetM.choose, NonDetM.assume, NonDetM.pure, NonDetM.bind, StateT.lift, StateT.pure]
+
+
+abbrev succ' : StateT Int NonDetM Int :=
+  do
+    let x <- get
+    set (x + 1)
+    let y <- NonDetM.choose Int
+    NonDetM.assume (y > x)
+    return y
+
+example (P : _ -> Prop) i : P ((succ' i).tp) := by
+  simp [succ', bind, pure, NonDetM.choose, NonDetM.assume, NonDetM.pure, NonDetM.bind]
+  simp [StateT.bind, StateT.get, pure, NonDetM.pure, liftM, monadLift, MonadLift.monadLift]
+  simp [succ', bind, pure, NonDetM.choose, NonDetM.assume, NonDetM.pure, NonDetM.bind, StateT.lift, StateT.pure]
+
+
+  sorry
+
+#reduce! ((succ 5).tp)
+
+#reduce (succ 5).val (by
+  dsimp [succ, bind, pure, NonDetM.choose, NonDetM.assume, NonDetM.pure, NonDetM.bind]
+  exact ⟨6, PLift.up (by omega), ()⟩)
+
+
+
+
+
+instance NonDetM.Setoid : Setoid (NonDetM α) where
+  r := fun ⟨tp₁, val₁⟩ ⟨tp₂, val₂⟩ => ∃ f : tp₁ -> tp₂, f.Bijective ∧ ∀ x, val₁ x = val₂ (f x)
+  iseqv := {
+    refl := by
+      rintro ⟨tp, val⟩; simp; exists id; simp; exact Function.bijective_id
+    symm := by
+      rintro ⟨tp₁, val₁⟩ ⟨tp₂, val₂⟩; simp; intro f bij valf
+      exists f.surjInv bij.2; constructor
+      { refine Function.bijective_iff_has_inverse.mpr ?_; exists f; constructor
+        { refine Function.RightInverse.leftInverse ?_
+          exact Function.rightInverse_surjInv bij.right }
+        refine Function.LeftInverse.rightInverse ?_
+        exact Function.leftInverse_surjInv bij }
+      simp [valf, Function.surjInv_eq]
+    trans := by
+      rintro ⟨tp₁, val₁⟩ ⟨tp₂, val₂⟩ ⟨tp₃, val₃⟩; simp; intros f₁ bij₁ valf₁ f₂ bij₂ valf₂
+      exists f₂ ∘ f₁; constructor
+      { exact Function.Bijective.comp bij₂ bij₁ }
+      aesop
+  }
+
+lemma bind_eq {x y : NonDetM α} {f g : α → NonDetM β} :
+  x ≈ y ->
+  (∀ a, f a ≈ g a) ->
+  (NonDetM.bind x f) ≈ (NonDetM.bind y g) := by
+  rcases x with ⟨tp₁, val₁⟩
+  rcases y with ⟨tp₂, val₂⟩
+  rintro ⟨eq, bij, valf⟩
+  simp [HasEquiv.Equiv, Setoid.r]; intro r
+  rcases Classical.skolem.mp r with ⟨fr, fbij⟩
+  simp [NonDetM.bind]
+  admit
+
+
+abbrev LawfullNonDetM α := Quotient (@NonDetM.Setoid α)
+
+variable {α : Type u} {β : Type v}
+
+abbrev LawfullNonDetM.mk : NonDetM α -> LawfullNonDetM α := Quotient.mk NonDetM.Setoid
+
+def LawfullNonDetM.pure (x : α) := NonDetM.pure x |> LawfullNonDetM.mk
+
+noncomputable def LawfullNonDetM.bind (x : LawfullNonDetM α) (f : α → LawfullNonDetM β) : LawfullNonDetM β :=
+  Quotient.liftOn x (fun x => Quotient.liftOnFun f (fun f => NonDetM.bind x f))
+  (by
+   intro a b eq; simp; sorry ) |> LawfullNonDetM.mk
