LoL/MProp/NonDetT.lean
@@ -1,0 +1,160 @@
+import Mathlib.Logic.Function.Basic
+import Aesop
+import LoL.QuotientExtra
+import LoL.Meta
+import LoL.MProp.HoareTriples
+
+universe u v w
+
+section Outcomes
+
+variable {m : Type u -> Type v} {l : Type u} [Monad m] [PartialOrder l] [MPropPartialOrder m l]
+
+def isReachable {α : Type u} (out : α) (x : m α) :=
+  ¬ mtriple (pure True) x fun x => pure (x ≠ out)
+
+def outcomes {α : Type u} (x : m α) := { out : α // isReachable (l := l) out x }
+
+end Outcomes
+
+section NonDetermenisticTransformer
+
+structure NonDetT (m : Type u -> Type v) (l : Type u)
+  [Monad m] [PartialOrder l] [MPropPartialOrder m l] (α : Type u) where
+  tp  : Type w
+  sem : tp → m α
+
+variable {m : Type u -> Type v} {l : Type u} {α β : Type u} [Monad m] [PartialOrder l] [MPropPartialOrder m l]
+
+def NonDetT.pure (x : α) : NonDetT m l α := ⟨PUnit, fun _ => return x⟩
+
+def NonDetT.bind (x : NonDetT m l α) (f : α → NonDetT m l β) : NonDetT m l β :=
+  ⟨
+    (tp : x.tp) × (out : outcomes (l := l) (x.sem tp)) × (f out.val).tp,
+    fun ⟨_, out, tp'⟩ => f out.val |>.sem tp'
+  ⟩
+
+def NonDetT.pick (τ : Type u) : NonDetT m l τ := ⟨τ, Pure.pure⟩
+
+structure PropType (α : Prop) : Type w where
+  prf : α
+
+def NonDetT.assume (as : Prop) : NonDetT m l PUnit := ⟨PropType as, fun _ => return .unit⟩
+
+instance : Monad (NonDetT m l) where
+  pure := .pure
+  bind := .bind
+
+instance foo : MonadLift m (NonDetT m l) where
+  monadLift := fun x => ⟨PUnit, fun _ => x⟩
+
+class MonadInfNonDet (m : Type u → Type v) where
+  pick : (τ : Type u) → m τ
+  assume : Prop → m PUnit
+
+export MonadInfNonDet (pick assume)
+
+instance : MonadInfNonDet (NonDetT m l) where
+  pick   := .pick
+  assume := .assume
+
+theorem pick_tp (τ : Type u) : (pick (m := NonDetT m l) τ).tp = τ := rfl
+theorem assume_tp (as : Prop) : (assume (m := NonDetT m l) as).tp = PropType as := rfl
+theorem lift_tp {α : Type u} (x : m α) : (liftM (n := NonDetT m l) x).tp = PUnit := rfl
+
+theorem pick_isReachable τ out t [LawfulMonad m] :
+  isReachable out ((pick (m := NonDetT m l) τ).sem t) = (out = t) := by
+    simp [isReachable, pick, NonDetT.pick]
+    rw [mtriple_pure]; constructor
+    { contrapose; simp; intro neq;
+      solve_by_elim [MPropPartialOrder.μ_ord_pure] }
+    rintro rfl; simp; intro
+    apply MPropPartialOrder.μ_nontriv (m := m)
+    apply le_antisymm <;> try assumption
+    apply MPropPartialOrder.μ_bot
+
+theorem pick_outcomes [LawfulMonad m] (τ : Type u) (t : τ) :
+  outcomes ((pick (m := NonDetT m l) τ).sem t) = { out // out = t } := by
+    simp [outcomes, pick_isReachable]
+
+theorem pick_outcomesE [LawfulMonad m] (τ : Type u) (t : τ)
+  (out : outcomes ((pick (m := NonDetT m l) τ).sem t)) :
+  out.val = t := by
+    have: isReachable out.val ((pick (m := NonDetT m l) τ).sem t) := by apply out.prop
+    rwa [pick_isReachable] at this
+
+instance NonDetM.Setoid : Setoid (NonDetT m l α) where
+  r := fun ⟨tp₁, val₁⟩ ⟨tp₂, val₂⟩ => ∃ f : tp₁ -> tp₂, f.Bijective ∧ ∀ x, val₁ x = val₂ (f x)
+  iseqv := {
+    refl := by
+      rintro ⟨tp, val⟩; simp; exists id; simp; exact Function.bijective_id
+    symm := by
+      rintro ⟨tp₁, val₁⟩ ⟨tp₂, val₂⟩; simp; intro f bij valf
+      exists f.surjInv bij.2; constructor
+      { refine Function.bijective_iff_has_inverse.mpr ?_; exists f; constructor
+        { refine Function.RightInverse.leftInverse ?_
+          exact Function.rightInverse_surjInv bij.right }
+        refine Function.LeftInverse.rightInverse ?_
+        exact Function.leftInverse_surjInv bij }
+      simp [valf, Function.surjInv_eq]
+    trans := by
+      rintro ⟨tp₁, val₁⟩ ⟨tp₂, val₂⟩ ⟨tp₃, val₃⟩; simp; intros f₁ bij₁ valf₁ f₂ bij₂ valf₂
+      exists f₂ ∘ f₁; constructor
+      { exact Function.Bijective.comp bij₂ bij₁ }
+      aesop
+  }
+
+lemma bind_eq {x y : NonDetT m l α} {f g : α → NonDetT m l β} :
+  x ≈ y ->
+  (∀ a, f a ≈ g a) ->
+  (NonDetT.bind x f) ≈ (NonDetT.bind y g) := by
+  rcases x with ⟨tp₁, val₁⟩
+  rcases y with ⟨tp₂, val₂⟩
+  rintro ⟨eq, bij, valf⟩
+  simp only [HasEquiv.Equiv, Setoid.r]; intro r
+  rcases Classical.skolem.mp r with ⟨eqf, bijf⟩; clear r
+  simp only [NonDetT.bind]
+  exists by
+    intro ⟨t, outs, ftp⟩
+    -- intros ⟨⟩
+
+
+
+
+notation "NonDetT" t => NonDetT t _
+
+end NonDetermenisticTransformer
+
+
+section Example
+
+open TotalCorrectness
+
+abbrev myM := NonDetT (StateT Nat (ExceptT String Id))
+
+def ex : myM ℕ :=
+  do
+    let x ← pick ℕ
+    let y ← pick ℕ
+    set (x + y)
+    assume (x > y)
+    pure (x + y)
+
+
+-- set_option pp.explicit true
+
+example (P : _ -> Prop) : P (ex) := by
+  dsimp [ex, bind, pure]
+  unfold InfNonDetT.bind InfNonDetT.pure;
+  simp [set]
+  simp [pick_tp, assume_tp, lift_tp, pick_outcomesE]
+  -- #check @pick_outcomes (StateT Nat (ExceptT String Id)) _ inferInstance inferInstance inferInstance inferInstance ℕ
+  -- simp []
+  have : ∀ (tp : ℕ) (out : outcomes ((@pick myM instMonadInfNonDetInfNonDetT ℕ).sem tp)), out.val = tp := by
+    intro; simp [pick_outcomesE]
+
+
+
+#reduce! ex
+
+end Example
