LoL/QuotientExtra.lean
@@ -1,0 +1,26 @@
+universe u v w
+
+namespace Quotient
+
+variable {α : Sort u} {β : Sort v} {γ : Sort w}
+
+noncomputable def Quotient.rep {s : Setoid α} (q : Quotient s) : α :=
+  Classical.choose (Quotient.exists_rep q)
+
+protected noncomputable abbrev liftOnFun
+  {s : Setoid α} (q : γ -> Quotient s) (f : (γ -> α) → β) : β :=
+  f (fun x => Quotient.rep (q x))
+
+@[simp]
+theorem liftOnFun_correct {s : Setoid α} (q : γ -> α) (f : (γ -> α) → β) :
+  ((a b : γ -> α) → (∀ x, a x ≈ b x) → f a = f b) ->
+  Quotient.liftOnFun (fun x => Quotient.mk s (q x)) f = f q := by
+  intro h
+  apply h; simp [Quotient.rep]; intro y
+  have h := fun x => Classical.choose_spec (@Quotient.exists_rep _ s x)
+  exact exact (h (Quotient.mk s (q y)))
+
+
+
+
+end Quotient
