LoL/SpecMonad.lean
@@ -20,8 +20,8 @@ export LawfulMonadLift (lift_pure lift_bind)
 
 alias EffectObservation := LawfulMonadLift
 
-class abbrev SpecMonad (m : Type u -> Type w) (w : Type u -> Type v) [Monad m] :=
-  MonadOrder w, MonadLiftT m w, EffectObservation m w
+-- class abbrev SpecMonad (m : Type u -> Type w) (w : Type u -> Type v) [Monad m] :=
+--   MonadOrder w, MonadLiftT m w, EffectObservation m w
 
 /-
   Spec for myM :
