README.md
@@ -2,6 +2,11 @@
 
 ## Interface:
 
+### Specifiying effects 
+- if `P : m Prop`, `c : m A` and `Q : A -> m Prop` then `{ P } c { Q }` is LoL specification
+- to specify effects like thorow we should write `{ P } c { fun _ => throw e }`
+  - `\mu := String -> Prop` st `\mu s := (. = s)`
+
 ### Total functions
 
 ```lean4
@@ -21,4 +26,3 @@ first you prove the following total Hoare-logic
 lemma foo_spec (P : m Prop) (Q : a -> m Prop) : { P } foo { x, Q x } := ...
 ```
 This means `foo` terminates, providing `P`. This should give you a total function `foo : P -> m a`. We can run it in Lean by `foo sorryAx`.
-
